more

Weidenbach_Book/IsaFoR/Ceta_SAT_Code.thy
@@ -12,9 +12,19 @@ lemma [code del]: "mset xs - mset ys = mset (fold remove1 ys xs)"
   nat_of_integer *)
   in SML module_name Ceta file "code/test.sml" *)
 
-lemma plain_name_hnr[sepref_fr_rules]:
-  \<open>(return o plain_name, RETURN o plain_name) \<in> id_assn\<^sup>k \<rightarrow>\<^sub>a id_assn\<close>
-  by (sepref_to_hoare) sep_auto
+lemma list_assn_pure_conv':
+  \<open>list_assn (\<lambda>a c. \<up> (c = a)) = pure (\<langle>Id\<rangle>list_rel)\<close>
+  unfolding pure_def[symmetric] list_assn_pure_conv
+  pair_in_Id_conv[symmetric]
+  ..
+
+lemma id_assn_eq_iff: \<open>id_assn a b = (\<up> (a = b))\<close>
+  unfolding pure_def by auto
+
+
+lemma id_assn_alt': \<open>(\<lambda>a c. \<up> (c = a)) = id_assn\<close>
+  unfolding pure_def[symmetric] pair_in_Id_conv[symmetric]
+  by auto
 
 abbreviation char_assn :: \<open>char \<Rightarrow> char \<Rightarrow> assn\<close> where
   \<open>char_assn \<equiv> id_assn\<close>
@@ -22,65 +32,76 @@ abbreviation char_assn :: \<open>char \<Rightarrow> char \<Rightarrow> assn\<clo
 abbreviation string_assn where
   \<open>string_assn \<equiv> list_assn char_assn\<close>
 
+lemma unfold_to_id_assn:
+  \<open>option_assn id_assn = id_assn\<close>
+  \<open>string_assn = id_assn\<close>
+  \<open>(\<lambda>a c. \<up> (c = a)) = id_assn\<close>
+  \<open>(\<lambda>a c. emp) = unit_assn\<close>
+     apply (intro ext; auto simp: option_assn_alt_def list_assn_pure_conv' id_assn_eq_iff
+      split: option.splits; fail)
+    apply (intro ext; auto simp: option_assn_alt_def list_assn_pure_conv; fail)
+   apply (intro ext; auto simp: option_assn_alt_def list_assn_pure_conv id_assn_eq_iff; fail)
+  apply (intro ext; auto simp: option_assn_alt_def list_assn_pure_conv id_assn_eq_iff; fail)
+  done
+
+lemma plain_name_hnr[sepref_fr_rules]:
+  \<open>(return o plain_name, RETURN o plain_name) \<in> id_assn\<^sup>k \<rightarrow>\<^sub>a id_assn +\<^sub>a id_assn\<close>
+  supply plain_name.simps[simp del]
+  unfolding sum_assn_id
+  by (sepref_to_hoare) sep_auto
+
 abbreviation cert_result_assn :: \<open>cert_result \<Rightarrow> cert_result \<Rightarrow> assn\<close> where
   \<open>cert_result_assn \<equiv> id_assn\<close>
 
 definition parse_xtc_plain_name where
   \<open>parse_xtc_plain_name = parse_xtc plain_name\<close>
 
-lemma list_assn_pure_conv'[simp]:
-  \<open>list_assn (\<lambda>a c. \<up> (c = a)) = pure (\<langle>Id\<rangle>list_rel)\<close>
-  unfolding pure_def[symmetric] list_assn_pure_conv
-  pair_in_Id_conv[symmetric]
-  ..
-lemma id_assn_sting_pure[simp]:
-  \<open>id_assn x xi = \<up>(x = xi)\<close>
-  unfolding pure_def by auto
+
+definition pure_fun_assn :: \<open>('a \<Rightarrow> 'b) \<Rightarrow> ('a \<Rightarrow> 'b) \<Rightarrow> assn\<close> where
+  \<open>pure_fun_assn = id_assn\<close>
+
+definition fun_comp where
+  \<open>fun_comp f x = f x\<close>
+
+lemma fun_comp_hnr:
+  \<open>(uncurry (return oo (\<lambda>f x. f x)), uncurry (RETURN oo fun_comp)) \<in>
+     pure_fun_assn\<^sup>k *\<^sub>a id_assn\<^sup>k \<rightarrow>\<^sub>a id_assn\<close>
+  by sepref_to_hoare (sep_auto simp: pure_fun_assn_def fun_comp_def)
+
+lemma fun_comp_list_hnr:
+  \<open>(uncurry (return oo (\<lambda>f x. f x)), uncurry (RETURN oo fun_comp)) \<in>
+     pure_fun_assn\<^sup>k *\<^sub>a (list_assn id_assn)\<^sup>k \<rightarrow>\<^sub>a list_assn id_assn\<close>
+  by sepref_to_hoare (sep_auto simp: pure_fun_assn_def fun_comp_def id_assn_eq_iff list_assn_pure_conv')
+
+
 
 definition input_assn
   :: \<open>((string, nat list) lab, string) input \<Rightarrow> ((string, nat list) lab, string) input \<Rightarrow> assn\<close>
 where
   \<open>input_assn = id_assn\<close>
 
-lemma id_assn_eq_iff: \<open>id_assn a b = (\<up> (a = b))\<close>
-  unfolding pure_def by auto
 
 lemma parse_xtc_plain_name_hnr[sepref_fr_rules]:
   \<open>(return o parse_xtc_plain_name, RETURN o (parse_xtc_plain_name)) \<in>
     string_assn\<^sup>k \<rightarrow>\<^sub>a (sum_assn string_assn input_assn)\<close>
-  by (sepref_to_hoare) (sep_auto elim!: sum_assn.elims simp: input_assn_def id_assn_eq_iff)
+  by (sepref_to_hoare) (sep_auto elim!: sum_assn.elims simp: input_assn_def id_assn_eq_iff
+      list_assn_pure_conv')
 
 
 lemma Error_hnr[sepref_fr_rules]:
   \<open>(return o Error, RETURN o Error) \<in> string_assn\<^sup>k \<rightarrow>\<^sub>a cert_result_assn\<close>
-  by (sepref_to_hoare) sep_auto
+  by (sepref_to_hoare) (sep_auto simp: list_assn_pure_conv')
 
 definition parse_claim_plain_name :: "string \<Rightarrow> string + ('a, 'b) claim" where
   \<open>parse_claim_plain_name = parse_claim plain_name\<close>
 
-lemma id_assn_id_assn_sum_rel[simp]:
-   \<open>id_assn +\<^sub>a (\<lambda>a c. \<up> (c = a)) = id_assn\<close>
-  unfolding pure_def[symmetric] pair_in_Id_conv[symmetric]
-  by auto
 
 lemma parse_claim_plain_name_hnr[sepref_fr_rules]:
   \<open>(return o parse_claim_plain_name, RETURN o (parse_claim_plain_name)) \<in>
     string_assn\<^sup>k \<rightarrow>\<^sub>a (sum_assn string_assn id_assn)\<close>
-  by (sepref_to_hoare) (sep_auto elim!: sum_assn.elims simp: input_assn_def id_assn_eq_iff)
-
-term parse_cert_problem
-
-lemma id_assn_alt': \<open>(\<lambda>a c. \<up> (c = a)) = id_assn\<close>
-  unfolding pure_def[symmetric] pair_in_Id_conv[symmetric]
-  by auto
-
-
-lemma unfold_to_id_assn:
-  \<open>option_assn id_assn = id_assn\<close>
-  \<open>string_assn = id_assn\<close>
-   apply (intro ext; auto simp: option_assn_alt_def split: option.splits; fail)
-  apply (intro ext; auto simp: option_assn_alt_def list_assn_pure_conv; fail)
-  done
+  unfolding sum_assn_id unfold_to_id_assn
+  by (sepref_to_hoare) (sep_auto elim!: sum_assn.elims
+      simp: input_assn_def id_assn_eq_iff list_assn_pure_conv')
 
 lemma parse_cert_problem_hnr[sepref_fr_rules]:
   \<open>(return o parse_cert_problem, RETURN o (parse_cert_problem)) \<in>
@@ -93,30 +114,54 @@ definition no_input_pb where
 
 lemma no_input_pb_hnr[sepref_fr_rules]:
   \<open>(uncurry0 (return no_input_pb), uncurry0 (RETURN no_input_pb)) \<in> unit_assn\<^sup>k \<rightarrow>\<^sub>a string_assn\<close>
-  by sepref_to_hoare sep_auto
+  by sepref_to_hoare (sep_auto simp: list_assn_pure_conv' id_assn_eq_iff)
 
 definition certify_prob where
   \<open>certify_prob = certify_cert_problem tp_impl
                Ceta_Verifier.dpp_impl ac_tp_impl
                Ceta_Verifier.ac_dpp_impl\<close>
 
-term check_cert
+definition check_cert_args where
+  \<open>check_cert_args = check_cert tp_impl Ceta_Verifier.dpp_impl ac_tp_impl
+                      Ceta_Verifier.ac_dpp_impl\<close>
 
 lemma certify_prob_hnr[sepref_fr_rules]:
-  \<open>(uncurry3 (return oooo certify_prob), uncurry3 (RETURN oooo certify_prob)) \<in>
-        bool_assn\<^sup>k *\<^sub>a input_assn\<^sup>k  *\<^sub>a id_assn\<^sup>k  *\<^sub>a id_assn\<^sup>k \<rightarrow>\<^sub>a cert_result_assn\<close>
-  by sepref_to_hoare (sep_auto simp: input_assn_def)
+  \<open>(uncurry3 (return oooo check_cert_args), uncurry3 (RETURN oooo check_cert_args)) \<in>
+        bool_assn\<^sup>k *\<^sub>a input_assn\<^sup>k  *\<^sub>a id_assn\<^sup>k  *\<^sub>a id_assn\<^sup>k \<rightarrow>\<^sub>a pure_fun_assn +\<^sub>a unit_assn\<close>
+  by sepref_to_hoare (sep_auto simp: input_assn_def unfold_to_id_assn pure_fun_assn_def
+      id_assn_eq_iff list_assn_pure_conv')
+
+lemma Certified_hnr[sepref_fr_rules]:
+  \<open>(uncurry0 (return Certified), uncurry0 (RETURN Certified)) \<in>
+   unit_assn\<^sup>k \<rightarrow>\<^sub>a cert_result_assn\<close>
+  by sepref_to_hoare (sep_auto)
+
+sepref_definition  certify_prob_code
+  is \<open>uncurry3 (RETURN oooo certify_prob)\<close>
+  :: \<open>bool_assn\<^sup>k *\<^sub>a input_assn\<^sup>k  *\<^sub>a id_assn\<^sup>k  *\<^sub>a id_assn\<^sup>k \<rightarrow>\<^sub>a cert_result_assn\<close>
+  supply fun_comp_list_hnr[sepref_fr_rules]
+  unfolding certify_prob_def certify_cert_problem_def check_cert_args_def[symmetric]
+    HOL_list.fold_custom_empty
+  apply (rewrite at \<open>Error(_  \<hole>)\<close> annotate_assn[where A = \<open>string_assn\<close>])
+  apply (rewrite at \<open>Error(\<hole>)\<close> fun_comp_def[symmetric])
+  by sepref
+
+declare certify_prob_code.refine[sepref_fr_rules]
 
 (* "bool \<Rightarrow> string option \<Rightarrow> (_,_)claim + string \<Rightarrow> string \<Rightarrow> cert_result" where *)
 sepref_definition certify_proof_code
   is \<open>uncurry3 (RETURN oooo certify_proof)\<close>
-  :: \<open>bool_assn\<^sup>k *\<^sub>a (option_assn string_assn)\<^sup>k *\<^sub>a (sum_assn id_assn string_assn)\<^sup>k *\<^sub>a string_assn\<^sup>k \<rightarrow>\<^sub>a id_assn\<close>
+  :: \<open>bool_assn\<^sup>k *\<^sub>a (option_assn string_assn)\<^sup>k *\<^sub>a (sum_assn id_assn string_assn)\<^sup>k *\<^sub>a string_assn\<^sup>k \<rightarrow>\<^sub>a
+      cert_result_assn\<close>
   supply[[goals_limit=1]]
   unfolding certify_proof_def parse_xtc_plain_name_def[symmetric]
     parse_claim_plain_name_def[symmetric] certify_prob_def[symmetric]
     no_input_pb_def[symmetric]
   by sepref
 
+lemma prod_assn_id_assn_id_assn:
+  \<open>id_assn *a id_assn = id_assn\<close>
+  by auto
 
 theorem certify_proof_code_sound:
   assumes ret: "certify_proof_code False (Some input_str) (Inr claim_str) proof_str = return Certified"
@@ -125,6 +170,8 @@ theorem certify_proof_code_sound:
     parse_claim plain_name claim_str = Inr claim \<and>
     desired_property input claim"
 proof -
+  have [simp]: \<open>id_assn a b = \<up>(a =b)\<close> for a b
+    by (auto simp: pure_def)
   have H:
     \<open><emp>
        certify_proof_code a b ba bb
@@ -135,7 +182,8 @@ proof -
                        bb)>\<close>
     for a b ba bb
     using certify_proof_code.refine
-    unfolding hfref_def
+    unfolding hfref_def unfold_to_id_assn sum_assn_id hfprod_fst_snd keep_drop_sels
+      prod_assn_id_assn_id_assn
     by (auto simp: unfold_to_id_assn hn_refine_def)
   have H:\<open>(h, as) \<Turnstile> emp \<and>
        Run.run (Heap_Monad.return Certified)
@@ -161,6 +209,10 @@ proof -
     by (auto simp: run.simps return_def Heap_Monad.heap_def)
 qed
 
+thm certify_proof_def
+thm check_cert_def
+thm certify_cert_problem_def
+thm certify_proof_def
 (*
   apply sepref_dbg_keep
       apply sepref_dbg_trans_keep
@@ -170,7 +222,7 @@ qed
 
 (* export_code certify_proof_code in Haskell module_name Ceta *)
 
-text \<open>Function that shoul be replaced @{term pre_logic_checker.check_valid_formula} 
+text \<open>Function that shoul be replaced @{term pre_logic_checker.check_valid_formula}
   @{term pre_logic_checker.check_valid_formula} is called by
   @{term pre_logic_checker.check_valid_formula} called by
   @{term pre_logic_checker.check_formula} called by
@@ -185,13 +237,15 @@ text \<open>Function that shoul be replaced @{term pre_logic_checker.check_valid
        @{term pre_termination_checker.check_termination_proof} called by
        @{term pre_termination_checker.check} called by
        @{term IA_locale.check_termination} called by
-       @{term check_cert}
+       @{term check_cert} called by
+       @{term certify_cert_problem}
 
 
      for @{term pre_logic_checker.safe_by_assertion_checker}, calls by
      @{term pre_art_checker.check_safety_proof} called by
      @{term pre_art_checker.check_safety} called by
-     @{term check_cert}
+     @{term check_cert} called by
+     @{term certify_cert_problem}
   \<close>
 
 end
